clientsum.bpl
@@ -18,7 +18,7 @@ requires (instanceof[suCli] == 2) ==> (fracSumOKRealSum[suCli] > 0.0) ;
 procedure UnpackClientSumOK(suCli:Ref, this:Ref);
 requires packedClientSumOK[this];
 requires fracClientSumOK[this] > 0.0;
-ensures sumClient[this] == suCli;
+requires sumClient[this] == suCli;
 // TODO add requires about parameters if needed
 ensures (instanceof[suCli] == 1) ==> (fracSumOKProxySum[suCli] > 0.0) ;
 ensures (instanceof[suCli] == 2) ==> (fracSumOKRealSum[suCli] > 0.0) ;
@@ -33,7 +33,7 @@ requires (instanceof[suCli] == 2) ==> (fracSumGreater0RealSum[suCli] > 0.0) ;
 procedure UnpackClientSumGreater0(suCli:Ref, this:Ref);
 requires packedClientSumGreater0[this];
 requires fracClientSumGreater0[this] > 0.0;
-ensures sumClient[this] == suCli;
+requires sumClient[this] == suCli;
 // TODO add requires about parameters if needed
 ensures (instanceof[suCli] == 1) ==> (fracSumGreater0ProxySum[suCli] > 0.0) ;
 ensures (instanceof[suCli] == 2) ==> (fracSumGreater0RealSum[suCli] > 0.0) ;
@@ -132,12 +132,9 @@ fracBasicFieldsProxySum[s] := 1.0;
 instanceof[s] := 1;
 // could keep the if like below
 // but I instead simplified it
-
 call UnpackBasicFieldsProxySum(realSum[s], sum[s], n[s], s);
 packedBasicFieldsProxySum[s] := false;
-
 call temp := calculateSumProxySum(s);
-
 call ConstructClientSum(s, client1);
 packedClientSumOK[client1] := false;
 call PackClientSumOK(s, client1);
@@ -145,6 +142,7 @@ packedClientSumOK[client1] := true;
 fracClientSumOK[client1] := 1.0;
 
 call ConstructClientSum(s, client2);
+
 packedClientSumOK[client2] := false;
 call PackClientSumOK(s, client2);
 packedClientSumOK[client2] := true;
@@ -196,7 +194,6 @@ call PackBasicFieldsProxySum(realSum[s2], sum[s2], n[s2], s2);
 packedBasicFieldsProxySum[s2] := true;
 fracBasicFieldsProxySum[s2] := 1.0;
 instanceof[s2] := 1;
-
 call UnpackBasicFieldsProxySum(realSum[s2], sum[s2], n[s2], s2);
 packedBasicFieldsProxySum[s2] := false;
 call temp1 := addOneToSumProxySum(s2);
@@ -231,3 +228,5 @@ packedClientSumGreater0[client4] := false;
 
 call temp2 := checkSumGreater0(client4);
 }
+
+
