simpleCellOneFracMinimal.bpl
@@ -1,6 +1,5 @@
 type Ref;
 const null: Ref;
-
 var val: [Ref]int;
 var next: [Ref]Ref;
 var packedPredNext: [Ref] bool;
@@ -10,8 +9,7 @@ var fracPredVal: [Ref] real;
  
 procedure ConstructSimpleCell(val1: int, next1: Ref, this: Ref)
 	modifies val, next;
-	ensures (val[this] == val1) && 
-		(next[this] == next1);
+	ensures (val[this] == val1) && (next[this] == next1);
 	ensures (forall y:Ref :: ( (y!=this) ==> (val[y] == old(val[y]) ) ) );
 	ensures (forall y:Ref :: ( (y!=this) ==> (next[y] == old(next[y]) ) ) );
 {
@@ -65,35 +63,28 @@ procedure main()
 	var a : Ref;
 	var b : Ref;
   	assume (a!=b) && (b!=c) && (c!=a);
-  
 	call ConstructSimpleCell(2, null, c);
 	packedPredVal[c] := false; 
 	call PackPredVal(2, c);
 	packedPredVal[c] := true;
 	fracPredVal[c] := 1.0;
-
 	call ConstructSimpleCell(2, c, a);
 	packedPredNext[a] := false;
 	call PackPredNext(c, a);
 	packedPredNext[a] := true;
 	fracPredNext[a] := 1.0;
 	fracPredVal[c] := fracPredVal[c] - 0.34;
-
 	call ConstructSimpleCell(3, c, b);
-
 	packedPredNext[b] := false;
 	call PackPredNext(c, b);
 	packedPredNext[b] := true;
 	fracPredNext[b] := 1.0;
 	fracPredVal[c] := fracPredVal[c] - 0.34;
-
 	call UnpackPredNext(c, a);
 	packedPredNext[a] := false;
-
+        fracPredVal[c] := fracPredVal[c] + 0.34
 	call UnpackPredNext(c, b);
 	packedPredNext[b] := false;
-
-	fracPredVal[c] := fracPredVal[c]+0.34+0.34;
-
+	fracPredVal[c] := fracPredVal[c] + 0.34;
 	call changeVal(c, 4);
 }
